feat(new_solutions): Add Ex1.

new_solutions/Ex1.dfy
@@ -1,24 +1,24 @@
-datatype uop = Neg 
-datatype bop = Plus | Minus 
+datatype uop = Neg
+datatype bop = Plus | Minus
 
 datatype aexpr =
-  Var(seq<nat>)
+    Var(seq<nat>)
   | Val(nat)
   | UnOp(uop, aexpr)
   | BinOp(bop, aexpr, aexpr)
- 
-datatype code = 
-  | VarCode(seq<nat>)  
-  | ValCode(nat)       
-  | UnOpCode(uop)      
-  | BinOpCode(bop)     
 
-function Serialize(a : aexpr) : seq<code> 
+datatype code =
+  | VarCode(seq<nat>)
+  | ValCode(nat)
+  | UnOpCode(uop)
+  | BinOpCode(bop)
+
+function Serialize(a : aexpr) : seq<code>
 {
   match a {
     case Var(s) => [ VarCode(s) ]
     case Val(i) => [ ValCode(i) ]
-    case UnOp(op, a1) => Serialize(a1) + [ UnOpCode(op) ]
+    case UnOp(op, a1) => Serialize(a1) + [ UnOpCode(op) ] // sequence
     case BinOp(op, a1, a2) => Serialize(a2) + Serialize(a1) + [ BinOpCode(op) ]
   }
 }
@@ -27,83 +27,273 @@ function Serialize(a : aexpr) : seq<code>
 /*
   Ex1.1
 */
-function Deserialize(cs : seq<code>) : seq<aexpr> 
+function Deserialize(cs: seq<code>): seq<aexpr>
 {
   DeserializeAux(cs, [])
 }
 
-function DeserializeAux(cs: seq<code>, ts: seq<aexpr>) : seq<aexpr>
+function DeserializeAux(cs: seq<code>, currAexp: seq<aexpr>): seq<aexpr>
 {
-  if (|cs| == 0)
-    then ts
-    else DeserializeAux(cs[1..], DeserializeCode(cs[0], ts))
+  if |cs| == 0 then
+    currAexp
+  else
+    match cs[0] {
+      case ValCode(i) => DeserializeAux(cs[1..], [Val(i)] + currAexp)
+      case VarCode(a) => DeserializeAux(cs[1..], [Var(a)] + currAexp)
+      case UnOpCode(op) => 
+        if |currAexp| < 1 then [] 
+        else 
+          DeserializeAux(cs[1..], [UnOp(op, currAexp[0])] + currAexp[1..])
+      case BinOpCode(op) =>
+        if |currAexp| < 2 then []
+        else 
+          DeserializeAux(cs[1..], [BinOp(op, currAexp[0], currAexp[1])] + currAexp[2..])
+    }
 }
-
-function DeserializeCode(c: code, ts: seq<aexpr>): seq<aexpr>
-{
-  match c {
-    case VarCode(s) => [ Var(s) ] + ts
-    case ValCode(i) => [ Val(i) ] + ts
-    case UnOpCode(uop) =>
-      if (|ts| < 1)
-        then []
-        else [ UnOp(uop, ts[0]) ] + ts[1..]
-    // Since Serialize already swaps the two values, we don't need to do it here
-    // Otherwise, not commutative binary operations might be misplaced.
-    case BinOpCode(bop) => 
-      if (|ts| < 2)
-        then []
-        else [ BinOp(bop, ts[0], ts[1]) ] + ts[2..]
-  }
-}
-
 
 /*
   Ex1.2
 */
-// lemma DeserializeProperty(e : aexpr)
-//   ensures Deserialize(Serialize(e)) == [ e ]
-// {
- 
-// }
+lemma DeserializeProperty(e : aexpr)
+  ensures Deserialize(Serialize(e)) == [ e ]
+{ 
+  assert Serialize(e) + [] == Serialize(e);
+  calc{
+    Deserialize(Serialize(e));
+    ==
+    DeserializeAux(Serialize(e), []);
+    ==
+    DeserializeAux(Serialize(e) + [], []);
+    == {DeserializeAuxProperty(e, [], []);}
+    DeserializeAux([], [ e ] + []);
+    ==
+    [ e ];
 
-/*
-  Ex1.3
-*/
-// function SerializeCodes(cs : seq<code>) : seq<nat> 
-// {
+  }
+}
 
-// }
+lemma DeserializeAuxProperty(e : aexpr, cs: seq<code>, es: seq<aexpr>)
+  ensures DeserializeAux(Serialize(e)+ cs, es) == DeserializeAux(cs, [ e ] + es)
+{
+  match e {
+    case Val(i) =>
+      calc {
+        DeserializeAux(Serialize(e)+ cs, es);
+        ==
+        DeserializeAux(Serialize(Val(i))+ cs, es); // case
+        ==
+        DeserializeAux([ValCode(i)] + cs, es); // definition of Serialize
+        == 
+        DeserializeAux(cs, [Val(i)] + es); // definition of DeserializeAux
+        ==
+        DeserializeAux(cs, [ e ] + es); // case
 
-// function DeserializeCodes(ints : seq<nat>) : seq<code> {
+      }
+    case Var(a) =>
+      calc {
+        DeserializeAux(Serialize(e)+ cs, es);
+        ==
+        DeserializeAux(Serialize(Var(a))+ cs, es); // case
+        ==
+        DeserializeAux([VarCode(a)] + cs, es); // definition of Serialize
+        == 
+        DeserializeAux(cs, [Var(a)] + es); // definition of DeserializeAux
+        ==
+        DeserializeAux(cs, [ e ] + es); // case
+
+      }
+    case UnOp(op, a1) =>
+      assert Serialize(a1) + [ UnOpCode(op) ]+ cs == Serialize(a1) + ([ UnOpCode(op) ]+ cs);
+
+      calc {
+        DeserializeAux(Serialize(e)+ cs, es);
+        ==
+        DeserializeAux(Serialize(UnOp(op, a1))+ cs, es); // case
+        == 
+        DeserializeAux(Serialize(a1) + [ UnOpCode(op) ]+ cs, es); // definition of serialize
+        == 
+        DeserializeAux(Serialize(a1) + ([ UnOpCode(op) ]+ cs), es); // seq properties
+        ==  {DeserializeAuxProperty(a1, [ UnOpCode(op) ]+ cs, es);}
+        DeserializeAux([ UnOpCode(op) ] + cs, [a1] + es); // Induction hypothesis
+        == 
+        DeserializeAux(cs, [ UnOp(op, a1) ] + es); // Def of deserializeAux
+        ==
+        DeserializeAux(cs, [ e ] + es); // Case
+
+      }
+    case BinOp(op, a1, a2) =>
+      assert Serialize(a2) + Serialize(a1) + [ BinOpCode(op) ] + cs == Serialize(a2) + (Serialize(a1) + [BinOpCode(op)] + cs); //why this might not hold?
+      assert Serialize(a1) + [ BinOpCode(op) ] + cs == Serialize(a1) + ([BinOpCode(op)] + cs); //why this might not hold?
+      assert [a1] + ([a2] + es) == [a1, a2] + es;
+      calc{
+        DeserializeAux(Serialize(e) + cs, es);
+        ==
+        DeserializeAux(Serialize(BinOp(op, a1, a2)) + cs, es); //Case
+        ==
+        DeserializeAux(Serialize(a2) + Serialize(a1) + [ BinOpCode(op) ] + cs, es); // Def of serialize
+        ==
+        DeserializeAux(Serialize(a2) + (Serialize(a1) + [ BinOpCode(op) ] + cs), es); // Seq props
+        ==        
+        DeserializeAux(Serialize(a1) + [ BinOpCode(op) ] + cs, [a2] + es); // Lemma
+        ==
+        DeserializeAux(Serialize(a1) + ([ BinOpCode(op) ] + cs), [a2] + es); // Seq props
+        == {DeserializeAuxProperty(a2, [ BinOpCode(op) ] + cs, es);}
+        DeserializeAux([ BinOpCode(op) ] + cs, [a1] + ([a2] + es)); // lemma. Why cant be proved?
+        ==
+        DeserializeAux([ BinOpCode(op) ] + cs, [a1, a2] + es); // Seq props
+        ==
+        DeserializeAux(cs, [BinOp(op, a1, a2) ]+ es); // Deserialize def
+
+      }
+  }
+
+}
+
+// /*
+//   Ex1.3
+// */
+function SerializeCodes(cs : seq<code>) : seq<nat> 
+{
   
-// }
+  if cs == [] then []
+  else 
+    match cs[0] {
+    case ValCode(i) => [0] + [ i ] + SerializeCodes(cs[1..])
+    case VarCode(s) => [1] + [|s|] + s + SerializeCodes(cs[1..])
+    case UnOpCode(op) => [2] + SerializeCodes(cs[1..])
+    case BinOpCode(op) => match op {case Plus => [3] case Minus => [4]} + SerializeCodes(cs[1..])
+  }
+}
+
+function DeserializeCodes(ints : seq<nat>) : seq<code> 
+
+ {
+  if |ints| == 0 then []
+  else
+    match ints[0]{
+      case 0 => if |ints| == 1 then [] else [ ValCode(ints[1]) ] + DeserializeCodes(ints[2..])
+      case 1 => if |ints| == 1 || |ints| < ints[1] + 2 then [] else [ VarCode(ints[2..ints[1]+2]) ] + DeserializeCodes(ints[ints[1]+2..]) // E.g. 13ABCX
+      case 2 => [ UnOpCode(Neg) ] + DeserializeCodes(ints[1..])
+      case 3 => [ BinOpCode(Plus) ] + DeserializeCodes(ints[1..]) //add the ugly condition here?
+      case 4 => [ BinOpCode(Minus) ] + DeserializeCodes(ints[1..])
+      case _ => []
+    }
+}
 
 
-/*
-  Ex1.4
-*/
-// lemma DeserializeCodesProperty(cs : seq<code>)
-//   ensures DeserializeCodes(SerializeCodes(cs)) == cs
-// {
-// }
+// /*
+//   Ex1.4
+lemma DeserializeCodesProperty(cs: seq<code>)
+  ensures  DeserializeCodes(SerializeCodes(cs)) == cs
+  
+{
+   if cs == [] {
+    calc {
+      DeserializeCodes(SerializeCodes(cs));
+      == // Def of serialize
+      DeserializeCodes([]);
+      == // Def of deserialize
+      [];
+      == // Case
+      cs;
+    }
+  }
+  else{
+    match cs[0] {
+      case ValCode(i) =>
+        calc{
+          DeserializeCodes(SerializeCodes([ValCode(i)] + cs[1..]));
+          == // By SerializeCodes def
+          DeserializeCodes([0] + [ i ] + SerializeCodes(cs[1..]));
+          == // By serializeCodes def
+          [ ValCode(i) ] + DeserializeCodes(SerializeCodes(cs[1..]));
+          == {DeserializeCodesProperty(cs[1..]);} // By induction hypothesis
+          [ ValCode(i) ] + cs[1..];
+          == // By case
+          [cs[0]] + cs[1..];
+          ==
+          cs;
+        }
+      case VarCode(s) =>
+      calc{
+        DeserializeCodes(SerializeCodes([VarCode(s)] + cs[1..]));
+        == // Def of serialize
+        DeserializeCodes([1] + [|s|] + s + SerializeCodes(cs[1..]));
+        == // Def of deserialize
+        [ VarCode(s) ] + DeserializeCodes(SerializeCodes(cs[1..]));
+        == // Induction hypothesis
+        [ VarCode(s) ] + cs[1..];
+        ==
+        cs;
+      }
+      case UnOpCode(Neg) =>
+      calc{
+        DeserializeCodes(SerializeCodes([UnOpCode(Neg)] + cs[1..]));
+        == // Def of serialize
+        DeserializeCodes([2] + SerializeCodes(cs[1..]));
+        == // Def of deserialize
+        [ UnOpCode(Neg) ] + DeserializeCodes(SerializeCodes(cs[1..]));
+        == // Induction hypothesis
+        [ UnOpCode(Neg) ] + cs[1..];
+        ==
+        cs;
+      }
+      case BinOpCode(Plus) =>
+      calc{
+        DeserializeCodes(SerializeCodes([BinOpCode(Plus)] + cs[1..]));
+        == // Def of serialize
+        DeserializeCodes([3] + SerializeCodes(cs[1..]));
+        == // Def of deserialize
+        [ BinOpCode(Plus) ] + DeserializeCodes(SerializeCodes(cs[1..]));
+        == // Induction hypothesis
+        [ BinOpCode(Plus) ] + cs[1..];
+        ==
+        cs;
+      }
+      case BinOpCode(Minus) =>
+      calc{
+        DeserializeCodes(SerializeCodes([BinOpCode(Minus)] + cs[1..]));
+        == // Def of serialize
+        DeserializeCodes([4] + SerializeCodes(cs[1..]));
+        == // Def of deserialize
+        [ BinOpCode(Minus) ] + DeserializeCodes(SerializeCodes(cs[1..]));
+        == // Induction hypothesis
+        [ BinOpCode(Minus) ] + cs[1..];
+        ==
+        cs;
+      }
+    }
+  }
 
-/*
-  Ex1.5
-*/
-// function FullSerialize(e : aexpr) : seq<nat> {
- 
-// }
 
-// function FullDeserealize(nats : seq<nat>) : seq<aexpr> {
- 
-// }
+}
 
-/*
-  Ex1.6
-*/
-// lemma FullDeserealizeProperty(e : aexpr)
-//   ensures FullDeserealize(FullSerialize(e)) == [ e ]
-// {
-    
-// }
+// /*
+//   Ex1.5
+// */
+function FullSerialize(e : aexpr) : seq<nat> {
+  SerializeCodes(Serialize(e))
+}
+
+function FullDeserealize(nats : seq<nat>) : seq<aexpr> {
+ Deserialize(DeserializeCodes(nats))
+}
+
+// /*
+//   Ex1.6
+// */
+lemma FullDeserealizeProperty(e : aexpr)
+  ensures FullDeserealize(FullSerialize(e)) == [ e ]
+{
+  calc {
+      FullDeserealize(FullSerialize(e));
+      ==
+      FullDeserealize(SerializeCodes(Serialize(e)));
+      ==
+      Deserialize(DeserializeCodes(SerializeCodes(Serialize(e))));
+      == {DeserializeCodesProperty(Serialize(e));}
+      Deserialize(Serialize(e));
+      == {DeserializeProperty(e);}
+      [ e ];
+  }
+}
